\documentclass[12pt]{article}
%% Insert Commands in Preface.tex
\usepackage{sagetex}
\input{../Preface.tex}

\begin{document}

\thispagestyle{empty}

{\scshape Huang Linhang; Syx Pek; Qi Ji} \hfill {\scshape \large Differential Geometry} \hfill {\scshape Homework \#4}
 
\smallskip
\hrule
\bigskip
\section{Section 2.5}
\subsection*{Question 1}
The general recipe is to $(E, F, G) = (\langle \frac{ \partial x}{\partial u},\frac{ \partial x}{\partial u}\rangle, \langle\frac{ \partial x}{\partial u},\frac{ \partial x}{\partial v}\rangle,\langle\frac{ \partial x}{\partial v},\frac{ \partial x}{\partial v}\rangle)$.

Direct Computation shows,

\begin{enumerate}
    \begin{sagesilent}
        a,b,c,u,v = var('a,b,c,u,v')
        c1 = a*sin(u)*cos(v)
        c2 = b*sin(u)*sin(v)
        c3 = c*cos(u)
    \end{sagesilent}
    \item We have that 
    \begin{enumerate}
    \item $\frac{ \partial x}{\partial u} = (\sage{diff(c1,u)}, \sage{diff(c2, u)}, \sage{diff(c3,u)})$ 
    \item $\frac{ \partial x}{\partial v} = (\sage{diff(c1,v)}, \sage{diff(c2, v)}, \sage{diff(c3,v)})$
    \item $E = \sage{(diff(c1,u)^2 + diff(c2,u)^2 + diff(c3,u)^2).full_simplify()}$
    \item $F = \sage{(diff(c1,u)*diff(c1,v) + diff(c2,u)*diff(c2,v) + diff(c3,u)*diff(c3,v)).full_simplify()}$ 
    \item $G = \sage{(diff(c1,v)^2 + diff(c2,v)^2 + diff(c3,v)^2).full_simplify()}$
    \end{enumerate}

    \begin{sagesilent}
        a,b,c,u,v = var('a,b,c,u,v')
        c1 = a*u*cos(v)
        c2 = b*u*sin(v)
        c3 = u^2
    \end{sagesilent}
    \item We have that 
    \begin{enumerate}
    \item $\frac{ \partial x}{\partial u} = (\sage{diff(c1,u)}, \sage{diff(c2, u)}, \sage{diff(c3,u)})$ 
    \item $\frac{ \partial x}{\partial v} = (\sage{diff(c1,v)}, \sage{diff(c2, v)}, \sage{diff(c3,v)})$
    \item $E = \sage{(diff(c1,u)^2 + diff(c2,u)^2 + diff(c3,u)^2).full_simplify()}$
    \item $F = \sage{(diff(c1,u)*diff(c1,v) + diff(c2,u)*diff(c2,v) + diff(c3,u)*diff(c3,v)).full_simplify()}$ 
    \item $G = \sage{(diff(c1,v)^2 + diff(c2,v)^2 + diff(c3,v)^2).full_simplify()}$
    \end{enumerate}

    \begin{sagesilent}
        a,b,c,u,v = var('a,b,c,u,v')
        c1 = a*u*cosh(v)
        c2 = b*u*sinh(v)
        c3 = u^2
    \end{sagesilent}
    \item We have that 
    \begin{enumerate}
    \item $\frac{ \partial x}{\partial u} = (\sage{diff(c1,u)}, \sage{diff(c2, u)}, \sage{diff(c3,u)})$ 
    \item $\frac{ \partial x}{\partial v} = (\sage{diff(c1,v)}, \sage{diff(c2, v)}, \sage{diff(c3,v)})$
    \item $E = \sage{(diff(c1,u)^2 + diff(c2,u)^2 + diff(c3,u)^2).full_simplify()}$
    \item $F = \sage{(diff(c1,u)*diff(c1,v) + diff(c2,u)*diff(c2,v) + diff(c3,u)*diff(c3,v)).full_simplify()}$ 
    \item $G = \sage{(diff(c1,v)^2 + diff(c2,v)^2 + diff(c3,v)^2).full_simplify()}$
    \end{enumerate}

    \begin{sagesilent}
        a,b,c,u,v = var('a,b,c,u,v')
        c1 = a*sinh(u)*cos(v)
        c2 = b*sinh(u)*sin(v)
        c3 = c*cosh(u)
    \end{sagesilent}
    \item We have that 
    \begin{enumerate}
    \item $\frac{ \partial x}{\partial u} = (\sage{diff(c1,u)}, \sage{diff(c2, u)}, \sage{diff(c3,u)})$ 
    \item $\frac{ \partial x}{\partial v} = (\sage{diff(c1,v)}, \sage{diff(c2, v)}, \sage{diff(c3,v)})$
    \item $E = \sage{(diff(c1,u)^2 + diff(c2,u)^2 + diff(c3,u)^2).full_simplify()}$
    \item $F = \sage{(diff(c1,u)*diff(c1,v) + diff(c2,u)*diff(c2,v) + diff(c3,u)*diff(c3,v)).full_simplify()}$ 
    \item $G = \sage{(diff(c1,v)^2 + diff(c2,v)^2 + diff(c3,v)^2).full_simplify()}$
    \end{enumerate}
\end{enumerate}

\subsection*{Question 3}


\begin{sagesilent}
    a,b,c,u,v = var('a,b,c,u,v')
    c1 = 4*u/(u^2 + v^2 + 4)
    c2 = 4*v/(u^2 + v^2 + 4)
    c3 = 2*(u^2 + v^2)/(u^2 + v^2 + 4)
\end{sagesilent}

We have the parameterization 
$$x(u,v) = (\sage{c1}, \sage{c2}, \sage{c3}).$$

Hence,

\begin{enumerate}
\item $\frac{ \partial x}{\partial u} = (\sage{diff(c1,u)}, \sage{diff(c2, u)}, \sage{diff(c3,u)})$ 
\item $\frac{ \partial x}{\partial v} = (\sage{diff(c1,v)}, \sage{diff(c2, v)}, \sage{diff(c3,v)})$
\item $E = \sage{(diff(c1,u)^2 + diff(c2,u)^2 + diff(c3,u)^2).full_simplify()}$
\item $F = \sage{(diff(c1,u)*diff(c1,v) + diff(c2,u)*diff(c2,v) + diff(c3,u)*diff(c3,v)).full_simplify()}$ 
\item $G = \sage{(diff(c1,v)^2 + diff(c2,v)^2 + diff(c3,v)^2).full_simplify()}$
\end{enumerate}

\subsection*{Question 5}

We have the parameterization 
$$x(u,v) = (u,v, f(u,v)).$$

Hence,

\begin{enumerate}
\item $\frac{ \partial x}{\partial u} = (1, 0, \frac{ \partial f}{\partial u})$ 
\item $\frac{ \partial x}{\partial v} = (0,1, \frac{ \partial f}{\partial v})$
\end{enumerate}

And thus, $\frac{ \partial x}{\partial u} \times \frac{ \partial x}{\partial v} = (-\frac{ \partial x}{\partial u} ,-\frac{ \partial x}{\partial v}, 1)$
and so 
$$ A = \iint_Q |(-\frac{ \partial x}{\partial u} ,-\frac{ \partial x}{\partial v}, 1)| \mathrm dx \mathrm dy = \iint_Q \sqrt{\frac{ \partial x}{\partial u}^2 +\frac{ \partial x}{\partial v}^2 + 1^2} \mathrm dx \mathrm dy$$

\subsection*{Question 7}

The conditions translate to for all $a, b\in \mathbb R$ such that $a < b$.
\begin{align}
    \begin{split}
        \hat{E}(v) &= \int_a^b \sqrt{E(u,v)} \mathrm{d}u\\
        \hat{G}(u) &= \int_a^b \sqrt{G(u,v)} \mathrm{d}v
    \end{split}
\end{align}

are constant functions. Differentiation the first with respect to $v$, and the second with respect to $u$ yields the answer.

\subsection*{Question 9}


We consider the parameterization 
$$x(u,v) = (f(u)\cos(v), f(u)\sin(v), g(u))$$.

Hence,

\begin{enumerate}
\item $\frac{ \partial x}{\partial u} = (f'(u)\cos(v), f'(u)\sin(v), g'(u))$ 
\item $\frac{ \partial x}{\partial v} = (-f(u)\sin(v), f(u)\cos(v), 0)$
\item $E = f'(u)^2 + g'(u)^2$
\item $F = 0$ 
\item $G = 1$
\end{enumerate}

Swapping the variable names, $u \leftrightarrow v$ suffices.

\subsection*{Question 11}

Let \(S\) be a surface of revolution and \(C\) be its generating curve.
Let \(s\) be the arc length of \(C\) and denote by \(\rho = \rho(s)\) the distance to the rotation axis of the point of \(C\) corresponding to \(s\).

\begin{enumerate}
    \item[a.] \emph{(Pappus' Theorem.)} Show that the area of \(S\) is \[ 2\pi \int_0^1 \rho(s)\ ds, \]
        where \(l\) is the length of \(C\).
\end{enumerate}

\emph{Proof.}
Similarly to Example 4 of Sec. 2-3, we assume that the curve \(C\) lies in the \(xz\)-plane and the rotation axis is the \(z\)-axis.
Let \[\alpha(s) = (\rho(s), 0, h(s)), \quad 0 < s < l\] be parametrization of \(C\),
denote by \(\theta\) the rotation angle about the \(z\)-axis. Thus we obtain the map
\[ \mathbf{x}(\theta,s) = (\rho(s) \cos \theta, \rho(s) \sin \theta, h(s)) \]
which is a parametrisation \(U \to S\)
where \(U = \{(\theta,s): 0 < \theta < 2\pi , 0 < s < l\}\) is open.
Now we can compute
\begin{align*}
    \left\lvert \mathbf{x}_\theta \land \mathbf{x}_s \right\rvert
    &= \sqrt{\rho^2(s) (\rho'(s))^2 + \rho^2(s) (h'(s))^2} = \rho(s) \\
    \text{Area of } S
    &= \iint_U \left\lvert \mathbf{x}_\theta \land \mathbf{x}_s \right\rvert\ d\theta\ ds \\
    &= \int_0^l \int_0^2\pi \rho(s)\ d\theta\ ds \\
    &= 2\pi \int_0^l \rho(s)\ ds
\end{align*}
as desired.

\begin{enumerate}
    \item[b.] Apply part a to compute the area of a torus of revolution.
\end{enumerate}

\emph{Solution.}
Let \(R\) be the distance from the center of the tube to the center of the torus, and \(r\) be the radius of the tube.
The torus of revolution can be generated by the curve \(C\) parametrised by
\[ \alpha(s) = \left(R + r \cos\frac{s}{r},0,r\sin\frac{s}{r}\right), \quad 0 < s < 2\pi r.\]
In this case \(\rho(s) = R + r\cos\frac{s}{r}\),
so we have
\begin{align*}
    \text{Area of torus}
    &= 2\pi \int_0^{2\pi r} R + r\cos \frac{s}{r}\ ds \\
    &= 2\pi \left[ Rs + r^2\sin\frac{s}{r} \right]_0^{2\pi r} \\
    &= 4\pi^2 Rr.
\end{align*}


\section{Section 3.2}
\subsection*{Question 1}

Show that at a hyperbolic point, the principal directions bissect the asymptotic directions.

\emph{Proof.}
Let \(p\) be a hyperbolic point and let \(v\) be an asymptotic direction with angle \(\theta\) from \(e_1\),
where we write \(v\) as
\[ v = e_1\cos\theta + e_2\sin\theta. \]
As \(v\) is asymptotic by Euler's formula we have
\[ 0 = \mathrm{II}_p(v) = k_1 \cos^2\theta + k_2 \sin^2\theta. \]
Since we have the identities \(\cos(\pi-\theta) = -\cos\theta\) and \(\sin(\pi-\theta) = \sin(\theta)\)
we have
\[ v' = e_1\cos(\pi-\theta) + e_2\sin(\pi-\theta) \]
is also asymptotic.
Now we see that \(e_2\) bisects \(v\) and \(v'\).

\subsection*{Question 3}

Let \(C\subset S\) be a regular curve on a surface \(S\) with Gaussian curvature \(K>0\).
Show that the curvature \(k\) of \(C\) at \(p\) satisfies \[ k\geq \min(|k_1|,|k_2|),\]
where \(k_1\) and \(k_2\) are the principal curvatures of \(S\) at \(p\).

\emph{Proof.}
WLOG suppose the \(S\) is oriented such that both \(k_1, k_2\) are positive,
furthermore for simplicity suppose \(0 < k_1 < k_2\).
Note that \(k = k_n + k\sin\theta\) so \(k \geq k_n\),
it suffices to prove that \(k_n\geq \min(k_1,k_2)\).
Let \(v\) be the tangent of the curve \(C\) at \(p\), then
\[ v = e_1 \cos\theta + e_2 \sin\theta \]
for some angle \(\theta\).
By Euler's formula we have
\[ k_n = k_1 \cos^2(\theta) + k_2\sin^2(\theta). \]
Putting everything together we have
\[ k \geq k_n = k_1 \cos^2(\theta) + k_2\sin^2(\theta) \geq k_1 \cos^2(\theta) + k_1\sin^2(\theta) = k_1 = \min(k_1, k_2). \]

\section{Section 3.3}

\subsection*{Question 1}

Show that at the origin \((0,0,0)\) of the hyperboloid \(z = axy\) we have \(K = -a^2\) and \(H = 0\).

\emph{Solution.}
We parametrize the hyperboloid
\[ \mathbf{x}(u,v) = (u,v,auv). \]
We compute the following at origin \((0,0,0)\)
\begin{align*}
    \mathbf{x}_u &= (1,0,av) \\
    \mathbf{x}_v &= (0,1,au) \\
    \mathbf{x}_{uu} &= \mathbf{0} \\
    \mathbf{x}_{uv} &= (0,0,a) \\
    \mathbf{x}_{vv} &= \mathbf{0} \\
    N &= \frac{\mathbf{x}_u\wedge \mathbf{x}_v}{|\mathbf{x}_u\wedge \mathbf{x}_v|} = (-av, -au, 1) \\
    e &= \langle N,\mathbf{x}_{uu}\rangle = 0 \\
    f &= \langle N,\mathbf{x}_{uv}\rangle = a \\
    g &= \langle N,\mathbf{x}_{vv}\rangle = 0 \\
    E &= \langle \mathbf{x}_u,\mathbf{x}_u\rangle = 1 + a^2v^2 = 1\\
    F &= \langle \mathbf{x}_u,\mathbf{x}_v\rangle = a^2uv = 0\\
    G &= \langle \mathbf{x}_v,\mathbf{x}_v\rangle = 1+a^2u^2 = 1\\
    K &= \frac{eg - f^2}{EG - F^2} \\
      &= -a^2 \\
    H &= \frac12 \frac{eG - 2fF + gE}{EG - F^2} = 0
\end{align*}

\subsection*{Question 3}
Determine the asymptotic curves of the catenoid
\begin{equation*}
    \mathbf{x}(u,v)= (\cosh{v}\cos{u},\cosh{v}\sin{u},v).
\end{equation*}

\textit{Solution.} We have \begin{align*}
    &\mathbf{x}_u= (-\cosh{v}\sin{u},\cosh{v}\cos{u},0),\\
    &\mathbf{x}_v= (\sinh{v}\cos{u},\sinh{v}\sin{u},1),\\
    &\mathbf{x}_{uu}= (-\cosh{v}\cos{u},-\cosh{v}\sin{u},0),\\
    &\mathbf{x}_{uv}= (-\sinh{v}\sin{u},\sinh{v}\cos{u},0),\\
    &\mathbf{x}_{vv}= (\cosh{v}\cos{u},\cosh{v}\sin{u},0).\\
\end{align*}
Hence, \begin{align*}
    N &= \frac{\mathbf{x}_u\wedge \mathbf{x}_v}{|\mathbf{x}_u\wedge \mathbf{x}_v|}\\
    &=\frac{(\cosh{v}\cos{u},\cosh{v}\sin{u},-\cosh{v}\sinh{v})}{(\cosh{v})^2}\\
    &=\frac{1}{\cosh{v}}(\cos{u},\sin{u},-\sinh{v}).
\end{align*}
Then\begin{align*}
    e &= \langle N,\mathbf{x}_{uu}\rangle = -1,\\
    f &= \langle N,\mathbf{x}_{uv}\rangle = 0,\\
    g &= \langle N,\mathbf{x}_{vv}\rangle = 1.\\
\end{align*}
This implies that the asymptotic directions correspond to $\langle u',v'\rangle$ satisfies \begin{align*}
    &e(u')^2 + 2fu'v' + g(v')^2 = 0\\
    \Rightarrow &-(u')^2 + (v')^2 = 0\\
    \Rightarrow & u'=v' \quad\text{or}\quad u'=-v'.
\end{align*}
This shows that the asymptotic curves are the traces of $v=u+a$ or $v=-u+b$ for some $a,b\in\mathbb{R}$, which are \begin{align*}
    &\alpha_a(u) = \mathbf{x}(u,u+a) = (\cosh{(u+a)}\cos{u},\cosh{(u+a)}\sin{u},u+a),\\
    &\beta_b(u) = \mathbf{x}(u,-u+b) = (\cosh{(-u+b)}\cos{u},\cosh{(-u+b)}\sin{u},-u+b).
\end{align*}
The collection of all $\alpha_a,\beta_b$ are all the asymptotic curves.

\subsection*{Question 9}
(Contact of Curves.) Define contact of order $\geq n$ ($n$ integer $\geq 1$) for regular curves in R3 with a common point $p$ and prove that\\
a. The notion of contact of order $\geq n$ is invariant by diffeomorphisms.\\
b. Two curves have contact of order $\geq 1$ at $p$ if and only if they are tangent at $p$.\\

\textit{Solution.} We say two surfaces $S$ and $\bar{S}$ with a common point $p$ to have contact of order $\geq n$ at $p$ if there exist parametrizations $\mathbf{x}(u, v)$ and $\mathbf{\tilde{x}}(u,v)$ in $p$ of $S$ and $\bar{S}$ such that the partial derivatives of $\mathbf{x}$ and $\mathbf{\tilde{x}}(u,v)$ agree up to order $n$.\\\\
a. Let $\psi:\mathbb{R}^3 \to \mathbb{R}^3$ be a diffeomorphism. Then for any partial derivative operator $\partial _I$ of order less than $n$ on $u-v$ space. Then \begin{equation*}
    \partial _I\psi(\mathbf{x}) = J_\psi(\mathbf{x})\partial _I\mathbf{x} = J_\psi(\mathbf{\tilde{x}})\partial _I\mathbf{\tilde{x}} = \partial _I\psi(\mathbf{\tilde{x}}),
\end{equation*}
where $J\psi(\cdot)$ is the Jacobian of $\psi$. This shows that the notion of contact is invariant by diffeomorphisms.\\\\
b. It is easy to see that the contact of order $\geq 1$ implies that the two surfaces are tangent. For the converse, we suppose $S$ and $\bar{S}$ are tangent at $p$ with parametrizations $\mathbf{x(u,v)}$ and $\mathbf{\tilde{x}}(u,v)$ respectively. Then at the point $p$, $\mathbf{\tilde{x}}_u, \mathbf{\tilde{x}}_v \in T_{\mathbf{x}}(p)$ we can write \begin{align*}
    &\mathbf{\tilde{x}}_u = a_1 \mathbf{x}_u + a_2 \mathbf{x}_v,\\
    &\mathbf{\tilde{x}}_v = b_1 \mathbf{x}_u + b_2 \mathbf{x}_v.\\
\end{align*}
Note that since $\mathbf{\tilde{x}}_u, \mathbf{\utilde{x}}_v$ are linearly independent, we have $a_1b_2-a_2b_1\neq 0$. Now let $w = \frac{b_2u-a_2v}{a_1b_2-a_2b_1}$, $l = \frac{b_1u-a_1v}{a_2b_1-a_1b_2}$ and $\mathbf{{y}}(w,l) = \mathbf{\tilde{x}}(u,v)$. Then \begin{align*}
    \mathbf{y}_w &= \frac{b_2}{a_1b_2-a_2b_1}\mathbf{\tilde{x}}_u-\frac{a_2}{a_1b_2-a_2b_1}\mathbf{\tilde{x}}_v=\mathbf{x}_u,\\
    \mathbf{y}_l &=
    \frac{b_1}{a_2b_1-a_1b_2}\mathbf{\tilde{x}}_u-\frac{a_1}{a_2b_1-a_1b_2}\mathbf{\tilde{x}}_v=\mathbf{x}_v.
\end{align*}
This shows that $S$ and $\bar{S}$ have contact of order $\geq 1$ at p. 

\subsection*{Question 15}
Give an example of a surface which has an isolated parabolic point $p$ (that is, no other parabolic point is contained in some neighborhood of $p$).

\textit{Solution.} Consider the graph $(x,y,x^4+x^2y^2+y^2)$. Let $h(x,y)=x^4+x^2y^2+y^2$. Then we have\begin{align*}
    K &= \frac{h_{xx}h_{yy}-(h_{xy})^2}{(1+h_x^2+h_y^2)^2} = \frac{24x^4-12x^2y^2+24x^2+4y^2}{(1+h_x^2+h_y^2)^2},\\
    e &= \frac{h_{xx}}{(1+h_x^2+h_y^2)^{1/2}}=\frac{12x^2+2y^2}{(1+h_x^2+h_y^2)^{1/2}},\\
    f &= \frac{h_{xy}}{(1+h_x^2+h_y^2)^{1/2}}=\frac{2x^2+2}{(1+h_x^2+h_y^2)^{1/2}},\\
    g &= \frac{h_{yy}}{(1+h_x^2+h_y^2)^{1/2}}=\frac{4xy}{(1+h_x^2+h_y^2)^{1/2}}.
\end{align*}
 Then $K=0$ only at $(0,0,0)$, at which $f$ is nonzero. This shows that the graph has an isolated parabolic point.n $K=0$ only at $(0,0,0)$, at which $f$ and $g$ are nonzero. This shows that the graph has an isolated parabolic point.
 
\subsection*{Question 19}
Obtain the asymptotic curves of the one-sheeted hyperboloid $x^2 + y^2 - z^2 = 1$.

\textit{Solution.} Note that the hyperboloid is a surface of revolution parametrized by \begin{equation*}
    \mathbf{x}(u,v) = (\phi(v)\cos{u},\phi(v)\sin{u},\psi(v)),
\end{equation*}
where $\phi(v) = \cosh{v},\psi(v)=\sinh{v}$ and $u\in(0,2\pi)$. Then\begin{align*}
    e &=  -\phi\psi'=-\cosh^2(v),\\
    f &= 0,\\
    g &= \psi'\phi''-\psi''\phi'=\cosh^2(v)-\sinh^2(v)=1.
\end{align*}
Then solving $e(u')^2 +2fu'v'+g(v')^2=0$, we have \begin{equation*}
    v'=u'\cosh(v) \qquad \text{or} \qquad v'=-u'\cosh(v).
\end{equation*}
Solving the ODE, we have \begin{equation*}
    u(t) = \pm \tan^{-1}(\sinh v(t)) + C,\qquad C\in \mathbb{R}
\end{equation*}
Hence, the asymptotic curves will be the trace of $\gamma_C(v) = (\pm\tan^{-1}( \sinh v)  + C,v), v\in R$. They are \begin{equation*}
    \alpha_C(v) = \mathbf{x}(\tan^{-1}( \sinh v)  + C,v)
\end{equation*} or \begin{equation*}
    \beta_C(v) = \mathbf{x}(-\tan^{-1}( \sinh v)  + C,v)
\end{equation*}

\subsection*{Question 21}
Let $S$ be a surface with orientation $N$. Let $V \subset S$ be an open set in $S$ and let $f : V \subset S \to R$ be any nowhere-zero differentiable function in $V$. Let $v_1$ and $v_2$ be two differentiable (tangent) vector fields in $V$ such that at each point of $V$, $v_1$ and $v_2$ are orthonormal and $v_1 \wedge v_2 = N$.\\
a. Prove that the Gaussian curvature $K$ of $V$ is given by \begin{equation*}
    K = \frac{\langle dfN(v_1)\wedge dfN(v_2),fN\rangle}{f^3}.
\end{equation*}
b. Apply the above result to show that iff is the restriction of \begin{equation*}
    \sqrt{\frac{x^2}{a^4}+\frac{y^2}{b^4}+\frac{z^2}{c^4}}
\end{equation*}
to the ellipsoid \begin{equation*}
    \frac{x^2}{a^2}+\frac{y^2}{b^2}+\frac{z^2}{c^2}=1,
\end{equation*}
 then the Gaussian curvature of the ellipsoid is\begin{equation*}
     K = \frac{1}{a^2b^2c^2}\frac{1}{f^4}.
\end{equation*}
 
\textit{Solution.} Since $f$ is a smooth function on $V=\mathbf{x}(u,v)$, if $\alpha'(0) = v_i = \frac{d}{dt}\mathbf{x}(\beta(t))|_{t=0}$, we have \begin{align*}
     dfN(v_i) &= \frac{d}{dt}f(\alpha(t))N(\alpha(t))\\
     &=(\frac{d}{dt}f(\alpha(t)))N(\alpha(t))|_{t=0} + f(\alpha(t))\frac{d}{dt}N(\alpha(t))|_{t=0}\\
     &=(\nabla(f\circ \mathbf{x}) \cdot \beta'(0))N + fdN(v_i).
\end{align*}
Hence, \begin{align*}
    &dfN(v_1) \wedge dfN(v_2) = (C_1N + fdN(v_1)) \wedge (C_2N + fdN(v_2))\\
    &= C_1N\wedge fdN(v_2) - C_2N \wedge fdN(v_1)+f^2(dN(v_1) \wedge dN(v_2))\\
    &= C_1N\wedge fdN(v_2) - C_2N \wedge fdN(v_1)+f^2\det(dN)(v_1 \wedge v_2)\\
    &= C_1N\wedge fdN(v_2) - C_2N \wedge fdN(v_1)+f^2\det(dN)N.
\end{align*}
Therefore, \begin{align*}
    dfN(v_1) \wedge dfN(v_2) \cdot fN &= C_1N\wedge fdN(v_2) \cdot fN - C_2N \wedge fdN(v_1) \cdot fN +f^2\det(dN)N \cdot fN\\
    &=f^3KN\cdot N = f^3K.
\end{align*}
Thus \begin{equation*}
    \frac{dfN(v_1) \wedge dfN(v_2) \cdot fN }{f^3}=K.
\end{equation*}
b. We know that \begin{align*}
    N(x,y,z) &= \frac{(\frac{2x}{a^2},\frac{2y}{b^2},\frac{2z}{c^2})}{|(\frac{2x}{a^2},\frac{2y}{b^2},\frac{2z}{c^2})|}\\
    &= \frac{(\frac{x}{a^2},\frac{y}{b^2},\frac{z}{c^2})}{|(\frac{x}{a^2},\frac{y}{b^2},\frac{z}{c^2})|}\\
    &=\frac{(\frac{x}{a^2},\frac{y}{b^2},\frac{z}{c^2})}{f(x,y,z)}.
\end{align*}
Therefore, $fN = (\frac{x}{a^2},\frac{y}{b^2},\frac{z}{c^2})$. Then \begin{align*}
    \frac{d}{dt}fN(\alpha(t))&= (\frac{x'(t)}{a^2},\frac{y'(t)}{b^2},\frac{z'(t)}{c^2})\\
    &=\begin{pmatrix} a^{-2}&&\\&b^{-2}&\\&&c^{-2}\end{pmatrix} \alpha'(t).
\end{align*}
Hence, $dfN(v_i) = \begin{pmatrix} a^{-2}&&\\&b^{-2}&\\&&c^{-2}\end{pmatrix}v_i$ and thus \begin{align*}
    K &= \frac{dfN(v_1) \wedge dfN(v_2) \cdot fN }{f^3}\\
    &= \det(dfN)\frac{(dfN^{-1})^T(v_1\wedge v_2) \cdot fN}{f^3}\\
    &=(abc)^{-2}\frac{(dfN^{-1})N \cdot fN}{f^3}\\
    &=(abc)^{-2}\frac{1}{f^3}\begin{pmatrix} a^{2}&&\\&b^{2}&\\&&c^{2}\end{pmatrix}\frac{(\frac{x}{a^2},\frac{y}{b^2},\frac{z}{c^2})}{f(x,y,z)} \cdot (\frac{x}{a^2},\frac{y}{b^2},\frac{z}{c^2})\\
    & = (abc)^{-2}\frac{1}{f^3}\frac{(x,y,z)}{f} \cdot (\frac{x}{a^2},\frac{y}{b^2},\frac{z}{c^2})\\
    &= \frac{1}{a^2b^2c^2}\frac{1}{f^4}
\end{align*}






\end{document}
