\documentclass[12pt]{article}
%% Insert Commands in Preface.tex
\usepackage{sagetex}
\input{../Preface.tex}

\begin{document}

\thispagestyle{empty}

{\scshape Huang Linhang; Syx Pek; Qi Ji} \hfill {\scshape \large Differential Geometry} \hfill {\scshape Homework \#6}

\smallskip
\hrule
\bigskip

\section*{Question 1}
\newcommand*{\inner}[1]{\left\langle #1\right\rangle}
\newcommand*{\TWO}{\mathrm{II}}
\newcommand*{\pdd}[2]{\frac{\partial #1}{\partial #2}}
\newcommand*{\pd}[1]{\pdd{}{#1}}
Please prove properties (i) to (v) of the covariance derivatives
assuming it arises from a tangential projection \(D_XY\),
note that \([X,Y]f= X(Yf)-Y(Xf)\).
\begin{enumerate}
    \item[(i)] \(\nabla_{X + f Y} Z = \nabla_X Z + f \nabla_Y Z\)
    \item[(ii)] \(\nabla_X (Y + Z) = \nabla_X Y + \nabla_X Z\)
    \item[(iii)] \(\nabla_X (fY) = (\nabla_X f) Y + f\nabla_X Y = X (f) Y + f \nabla_X Y\)
    \item[(iv)] \(\nabla_X \inner{Y,Z} = X\inner{Y,Z} = \inner{\nabla_X Y,Z} + \inner{Y, \nabla_X Z}\)
    \item[(v)] \([X,Y] = \nabla_X Y - \nabla_Y X\)
\end{enumerate}

\emph{Proof.}
\begin{enumerate}
    \item[(i)] This follows from property of directional derivative and bilinearity of \(\TWO\).
        \begin{align*}
            \nabla_{X + f Y} Z &= D_{X+ fY} Z - \TWO(X + fY,Z) N \\
                               &= D_X Z + f D_Y Z - \TWO(X,Z)N - f\TWO(Y,Z)N \\
                               &= \nabla_X Z + f \nabla_Y Z
        \end{align*}
    \item[(ii)] This holds for similar reasons.
        \begin{align*}
            \nabla_X (Y + Z) &= D_X(Y + Z) - \TWO(X, Y + Z) N \\
                             &= D_X Y + D_X Z - \TWO(X,Y) N - \TWO(X,Z) N \\
                             &= \nabla_X Y + \nabla_X Z
        \end{align*}

    \item[(iii)] Apply product rule of directional derivative and bilinearity of \(\TWO\), note that \(D_X f = \nabla_X f\) as \(f\) is real-valued.
        \begin{align*}
            \nabla_X (fY) &= D_X(f Y) - \TWO(X,fY) \\
                          &= (D_X f) Y + f (D_X Y) - f \TWO(X,Y) \\
                          &= (\nabla_X f) Y + f\nabla_X Y = X (f) Y + f \nabla_X Y
        \end{align*}

    \item[(iv)] For reasons similar to above, it suffices to show \(D_X \inner{Y,Z} = \inner{D_X Y,Z} + \inner{Y, D_X Z}\). We illustrate in the case that \(X,Y,Z\) are vector fields in \(\mathbb{R}^3\).
        \begin{align*}
            D_X \inner{Y,Z} &= \left. \frac{d}{dt}\inner{Y(\alpha(t)), Z(\alpha(t))} \right|_{t=0} \\
                            &= \left. \sum_{i=1}^3 Y^i Z^i \right|_{t=0} \\
                            &= \sum_{i=1}^3 \left.\frac{d Y^i}{dt} \right|_{t=0} Z^i
                            + \sum_{i=1}^3 Y^i \left.\frac{d Z^i}{dt} \right|_{t=0} \\
                            &= \inner{D_X Y, Z} + \inner{Y,D_X Z}
        \end{align*}
        where we appeal to product rule in the second-last line.
    \item[(v)] For smooth real-valued \(f\),
        \begin{align*}
            [X,Y]f &= X(Yf) - Y(Xf) \\
                   &= \sum_i X^i \pd{x^i} \left( \sum_j Y^j \pdd{f}{x^j} \right)
                    - \sum_j Y^j \pd{x^j} \left( \sum_i X^i \pdd{f}{x^i} \right) \\
                   &= \dots \\
                   &= \sum_{i,j} \left(X^i \pdd{Y^j}{x^i} - Y^i\pdd{X^j}{x^i}\right) \pdd{f}{x^j} \\
                   &= \left(D_X Y - D_Y X\right) f
        \end{align*}
\end{enumerate}

\section*{Question 2}

\begin{sagesilent}
forget()
M = Manifold(3, 'R^3', start_index=1)
c_spher.<a,b,h> = M.chart(r'a:(0,+oo) b:(0,pi):\theta h:(-oo,+oo)')
g = M.metric('g')
g[1,1], g[2,2], g[3,3] = 1, a^2, 1
nab = g.connection(name='Gamma', latex_name=r'\Gamma')
\end{sagesilent}

We have the parameterization
\begin{align*}
    x &= a\cos(\theta) \\
    y &= a\sin(\theta) \\
    z &= h
\end{align*}
Then the metric tensor is $\sage{g.display()}$ with non-vanishing Christoffel symbols
\begin{equation}
    \sage{nab.display()}
\end{equation}

Similarly, for the parameterization
\begin{align*}
    x &= r\sin(\phi)\cos(\theta) \\
    y &= r\sin(\phi)\sin(\theta) \\
    z &= \cos(\phi)
\end{align*}
\begin{sagesilent}
    forget()
    M = Manifold(3, 'R^3', start_index=1)
    c_spher.<r,th,ph> = M.chart(r'r:(0,+oo) th:(0,pi):\theta ph:(0,2*pi):\phi')
    g = M.metric('g')
    g[1,1], g[2,2], g[3,3] = 1, r^2 , (r*sin(th))^2
    nab = g.connection(name='Gamma', latex_name=r'\Gamma')
\end{sagesilent}
Then the metric tensor is $\sage{g.display()}$ with non-vanishing Christoffel symbols
\begin{equation}
    \sage{nab.display()}
\end{equation}


\section*{Question 3}
Let $e_1,e_2$ be a basis of $T_p(S)$ and $X=X^1e_1+X^2e_2, Y=Y^1e_1+Y^2e_2$. express $[X,Y]$ in terms of $X^i, Y^i$ and $e_i$.
\\
\textit{Solution.} We assume $e_1$ and $e_2$ can be smoothly extended into tangent fields on $S$. Then we have
\begin{align*}
    \nabla_XY &= \nabla_{X^1e_1+X^2e_2}(Y^1e_1+Y^2e_2)\\
    &=X^1\nabla_{e_1}Y^1e_1 + X^1\nabla_{e_1}Y^2e_2 +
    X^2\nabla_{e_2}Y^1e_1 + X^2\nabla_{e_2}Y^2e_2\\
    &=X^1Y^1\nabla_{e_1}e_1 + X^1Y^2\nabla_{e_1}e_2 +
    X^2Y^1\nabla_{e_2}e_1 + X^2Y^2\nabla_{e_2}e_2\\
    &~~+X^1e_1(Y^1)e_1 + X^1e_1(Y^2)e_2+ X^2e_2(Y^1)e_1+X^2e_2(Y^2)e_2;\\
    \nabla_YX &= \nabla_{Y^1e_1+Y^2e_2}(X^1e_1+X^2e_2)\\
    &=Y^1\nabla_{e_1}X^1e_1 + Y^1\nabla_{e_1}X^2e_2 +
    Y^2\nabla_{e_2}X^1e_1 + Y^2\nabla_{e_2}X^2e_2\\
    &=X^1Y^1\nabla_{e_1}e_1 + X^2Y^1\nabla_{e_1}e_2 +
    X^1Y^2\nabla_{e_2}e_1 + X^2Y^2\nabla_{e_2}e_2\\
    &~~+Y^1e_1(X^1)e_1 + Y^1e_1(X^2)e_2+ Y^2e_2(X^1)e_1+Y^2e_2(X^2)e_2;\\
\end{align*}
Therefore, $X^i,Y^j\neq 0$, we have \begin{align*}
    [X,Y] &= \nabla_XY - \nabla_YX\\
    &=(X^1Y^2\nabla_{e_1}e_2 +
    X^2Y^1\nabla_{e_2}e_1)-(Y^1X^2\nabla_{e_1}e_2 +
    Y^2X^1\nabla_{e_2}e_1)\\
    &~~+[X^1e_1(Y^1)e_1 + X^1e_1(Y^2)e_2+ X^2e_2(Y^1)e_1+X^2e_2(Y^2)e_2]\\
    &~~-[Y^1e_1(X^1)e_1 + Y^1e_1(X^2)e_2+ Y^2e_2(X^1)e_1+Y^2e_2(X^2)e_2]\\
    &=\det\begin{pmatrix}
         X^1&Y^1\\
         X^2&Y^2
    \end{pmatrix}[e_1,e_2]\\
    &~~+[X^1e_1(Y^1)+X^2e_2(Y^1)-Y^1e_1(X^1)-Y^2e_2(X^1)]e_1\\
    &~~+[X^1e_1(Y^2)+X^2e_2(Y^2)-Y^1e_1(X^2)-Y^2e_2(X^2)]e_2\\
\end{align*}

If $e_1 = \utilde{X}_u$ and $e_2 = \utilde{X}_v$, then we have $[e_1,e_2] = 0$ and hence
\begin{align*}
    [X,Y] &= [X^1e_1(Y^1)+X^2e_2(Y^1)-Y^1e_1(X^1)-Y^2e_2(X^1)]e_1\\
    &+[X^1e_1(Y^2)+X^2e_2(Y^2)-Y^1e_1(X^2)-Y^2e_2(X^2)]e_2\\
\end{align*}

\end{document}
